theories/typing/own.v
@@ -83,15 +83,15 @@ Section own.
     move=> ?????[|?]*; [by iIntros|]. rewrite/= {1}by_just_loc_ex.
     iIntros "#LFT #In (%&->& [%[Mt Own]] & Fr) Tok !>!>!>".
     iDestruct (ty_own_proph with "LFT In Own Tok") as "Upd"; [done|].
-    iApply (step_fupdN_wand with "Upd"). iIntros ">(%ξs & %q &%& PTok & Close) !>".
-    iExists ξs, q. iSplit; [done|]. iFrame "PTok Fr". iIntros "PTok".
+    iApply (step_fupdN_wand with "Upd"). iIntros ">(%ξl & %q &%& PTok & Close) !>".
+    iExists ξl, q. iSplit; [done|]. iFrame "PTok Fr". iIntros "PTok".
     iMod ("Close" with "PTok") as "[?$]". iExists vl. by iFrame.
   Qed.
   Next Obligation.
     move=> ?????[|?]*/=; [by iIntros|]. iIntros "#LFT #In #In' [%l[Mt Shr]] Tok !>!>".
     iDestruct (ty_shr_proph with "LFT In In' Shr Tok") as "> Upd"; [done|].
     iIntros "!>!>!>". iApply (step_fupdN_wand with "Upd").
-    iIntros ">(%ξs & %q &%& PTok & Close) !>". iExists ξs, q. iSplit; [done|].
+    iIntros ">(%ξl & %q &%& PTok & Close) !>". iExists ξl, q. iSplit; [done|].
     iFrame "PTok". iIntros "PTok". iMod ("Close" with "PTok") as "[Shr $]".
     iExists l. by iFrame.
   Qed.
@@ -212,13 +212,13 @@ Section typing.
     iFrame "Fr". iNext. iExists _. iFrame "Mt". by rewrite repeat_length.
   Qed.
 
-  Lemma type_new {As} (n: Z) n' x e pre E L C (T: _ As) :
+  Lemma type_new {Al} (n: Z) n' x e pre E L C (T: _ Al) :
     Closed (x :b: []) e → (0 ≤ n)%Z → n' = Z.to_nat n →
     (∀v: val, typed_body E L C (v ◁ own_ptr n' (↯ n') +:: T) (subst' x v e) pre) -∗
     typed_body E L C T (let: x := new [ #n] in e) (λ al, pre (() -:: al)).
   Proof. iIntros. subst. iApply type_let; by [apply type_new_instr|solve_typing]. Qed.
 
-  Lemma type_new_subtype {A As} (ty: _ A) n' (n: Z) (T: _ As) f e pre x E L C :
+  Lemma type_new_subtype {A Al} (ty: _ A) n' (n: Z) (T: _ Al) f e pre x E L C :
     Closed (x :b: []) e → (0 ≤ n)%Z → n' = Z.to_nat n → subtype E L f (↯ n') ty →
     (∀v: val, typed_body E L C (v ◁ own_ptr n' ty +:: T) (subst' x v e) pre) -∗
     typed_body E L C T (let: x := new [ #n] in e) (λ al, pre (f () -:: al)).
@@ -241,7 +241,7 @@ Section typing.
     { iIntros "!>_". iExists -[]. by iSplit. }
   Qed.
 
-  Lemma type_delete {A As Bs} (ty: _ A) n' (n: Z) p e E L C (T: _ As) (T': _ Bs) tr pre :
+  Lemma type_delete {A Al Bl} (ty: _ A) n' (n: Z) p e E L C (T: _ Al) (T': _ Bl) tr pre :
     Closed [] e → tctx_extract_ctx E L +[p ◁ own_ptr n' ty] T T' tr →
     n' = ty.(ty_size) → n = n' → typed_body E L C T' e pre -∗
     typed_body E L C T (delete [ #n; p ];; e) (tr (λ '(_ -:: al), pre al)).
@@ -250,8 +250,8 @@ Section typing.
     f_equal. fun_ext. by case.
   Qed.
 
-  Lemma type_letalloc_1 {A As Bs} (ty: _ A) (x: string) p e
-    (T: _ As) (T': _ Bs) tr pre E L C :
+  Lemma type_letalloc_1 {A Al Bl} (ty: _ A) (x: string) p e
+    (T: _ Al) (T': _ Bl) tr pre E L C :
     Closed [] p → Closed [x] e →
     tctx_extract_ctx E L +[p ◁ ty] T T' tr → ty.(ty_size) = 1 →
     (∀v: val, typed_body E L C (v ◁ own_ptr 1 ty +:: T') (subst x v e) pre) -∗
@@ -270,8 +270,8 @@ Section typing.
     f_equal. fun_ext. by case.
   Qed.
 
-  Lemma type_letalloc_n {A B B' As Bs} (ty: _ A) (tyr: _ B) (tyr': _ B')
-    gt st (T: _ As) (T': _ Bs) tr pre (x: string) p e E L C :
+  Lemma type_letalloc_n {A B B' Al Bl} (ty: _ A) (tyr: _ B) (tyr': _ B')
+    gt st (T: _ Al) (T': _ Bl) tr pre (x: string) p e E L C :
     Closed [] p → Closed [x] e → tctx_extract_ctx E L +[p ◁ tyr] T T' tr →
     typed_read E L tyr ty tyr' gt st →
     (∀v: val, typed_body E L C
